Util/Util.v
@@ -63,32 +63,28 @@ Section UPDT_ISTATE.
 
 End UPDT_ISTATE.
 
-Require Import Coq.Arith.PeanoNat.
+Definition eqb {T} (x y : T) : bool :=
+  if classicT (x = y) then
+    true
+  else
+    false.
+Infix "=?" := eqb (at level 70).
 
-Lemma eqb_id : forall n : nat, n =? n = true.
-intros.
-induction n.
+Lemma eqb_id {T} : forall n : T, n =? n = true.
+unfold eqb. intros.
+destruct (classicT (n = n)).
 easy.
-simpl.
-f_equal.
-easy.
-Qed.
-
-Lemma eqb_nid : forall n m : nat, n <> m -> n =? m = false.
-fix rec 1.
-intros.
-destruct n.
-destruct m.
-easy.
-easy.
-destruct m.
-easy.
-simpl in *.
-apply rec.
 congruence.
 Qed.
 
-Lemma differ_pointwise_trivial {A} (f : nat -> A) i x :
+Lemma eqb_nid {T} : forall n m : T, n <> m -> n =? m = false.
+intros. unfold eqb.
+destruct (classicT (n = m)).
+contradiction.
+easy.
+Qed.
+
+Lemma differ_pointwise_trivial {T A} (f : T -> A) i x :
   differ_pointwise f (fun j => if i =? j then x else f j) i.
 unfold differ_pointwise.
 intros.
