Core/ProgramRules.v
@@ -116,7 +116,8 @@ intros. psimpl.
 apply H. easy.
 Qed.
 
-Lemma lemCall {A Q S} {P : Relt VE VF} {m : E A} :
+Lemma lemCall {A} {P : Relt VE VF} {m : E A} :
+  forall Q S,
   Stable R Q ->
   Stable R S ->
   Commit i G P (CallEv m) Q ->
